examples/ITreePredicatesExample.v
@@ -22,7 +22,7 @@ From ITree Require Import
      ITreeFacts
      DijkstraMonad
      Eq.Paco2.
-.
+
 
 From Paco Require Import paco.
 
@@ -101,7 +101,7 @@ Section Proper.
    *)
   Instance proper_interpret_state {S R} : Proper ((@eq_itree (stateE S) R _ eq) ==> (@eq S) ==> (@eq_itree void1 (S * R) _ eq)) interpret_state.
   Proof.
-    ginit. pcofix CIH.
+    ginit. gcofix CIH.
     intros x y H0 x2 y0 H1.
     rewrite (itree_eta (interpret_state x x2)).
     rewrite (itree_eta (interpret_state y y0)).
@@ -235,7 +235,7 @@ Lemma state_independent : forall {S R} (t:itree (stateE S) R)
     forall s s', ('(s,x) <- interpret_state t s ;; ret x) ≅ ('(s,x) <- interpret_state t s' ;; ret x).
 Proof.
   intros S R.
-  ginit. pcofix CIH.
+  ginit. gcofix CIH.
   intros t H0 s s'.
   rewrite (itree_eta (interpret_state t s)).
   rewrite (itree_eta (interpret_state t s')).
@@ -267,7 +267,7 @@ Lemma state_independent_k : forall {S R U} (t:itree (stateE S) R)
     forall s s', (sx <- interpret_state t s ;; (k sx)) ≅ (sx <- interpret_state t s' ;; (k sx)).
 Proof.
   intros S R U.
-  ginit. pcofix CIH.
+  ginit. gcofix CIH.
   intros t H0 k INV s s'.
   rewrite (itree_eta (interpret_state t s)).
   rewrite (itree_eta (interpret_state t s')).
