secure_example/LabelledAsmHandler.v
@@ -1,0 +1,97 @@
+From Coq Require Import
+     Arith.PeanoNat
+     Lists.List
+     Strings.String
+     Morphisms
+     Setoid
+     RelationClasses.
+
+From ExtLib Require Import
+     Data.String
+     Structures.Monad
+     Structures.Traversable
+     Data.List.
+
+From ITree Require Import
+     ITree
+     ITreeFacts
+     Events.MapDefault
+     Events.State
+     Events.StateFacts
+     Core.Divergence
+     Dijkstra.TracesIT
+     Secure.SecureEqHalt
+     Secure.SecureEqEuttHalt
+     Secure.SecureEqWcompat
+     Secure.SecureEqBind
+     Secure.StrongBisimProper
+.
+
+From SecureExample Require Import 
+     LabelledImp
+     LabelledAsm
+     LabelledImpHandler.
+
+Import Monads.
+Import MonadNotation.
+Local Open Scope monad_scope.
+Local Open Scope string_scope.
+
+From Paco Require Import paco.
+
+(* Note that this definition sets considers all registers to be private *)
+
+Definition priv_asm (priv : privacy_map sensitivity_lat) (A : Type) (e : (Reg +' Memory +' (IOE sensitivity_lat)) A ) :=
+  match e with
+  | inl1 _ => Private
+  | inr1 (inl1 (Load x)) => priv x
+  | inr1 (inl1 (Store x _ )) => priv x
+  | inr1 (inr1 (LabelledPrint _ s _ ) ) => s
+  end.
+
+Definition low_reg_mem_equiv (priv : privacy_map sensitivity_lat) : (registers * memory) -> (registers * memory) -> Prop := fun '(reg1, mem1) '(reg2, mem2) => forall x, priv x = Public -> mem1 x = mem2 x.
+
+Definition reg_mem : Type := registers * memory.
+
+Definition low_eqit_secure_asmstate (b1 b2 : bool) (priv : var -> sensitivity) {R1 R2 : Type} (RR : R1 -> R2 -> Prop )
+           (m1 : stateT reg_mem (itree (IOE sensitivity_) R1) (m2 : stateT reg_mem (itree IOE) R2) : Prop :=
+  forall s1 s2, low_reg_mem_equiv priv s1 s2 -> eqit_secure sense_preorder priv_io (product_rel (low_reg_mem_equiv priv) RR) b1 b2 Public (m1 s1) (m2 s2).
+
+Lemma low_reg_mem_equiv_update_public:
+  forall (priv_map : privacy_map) (x : addr) (v : value),
+    priv_map x = Public ->
+    forall (reg1 : registers) (mem1 : memory) (reg2 : registers) (mem2 : memory),
+      low_reg_mem_equiv priv_map (reg1, mem1) (reg2, mem2) ->
+      low_reg_mem_equiv priv_map (reg1, update x v mem1) (reg2, update x v mem2).
+Proof.
+  intros priv_map x v Hx reg1 mem1 reg2 mem2 Hs.
+  red. red in Hs. intros. unfold update. rewrite Hs; auto.
+Qed.
+
+Lemma low_reg_mem_equiv_update_priv_l:
+  forall (priv_map : privacy_map) (x : addr) (v : value),
+    priv_map x = Private ->
+    forall (reg1 : registers) (mem1 : memory) (reg2 : registers) (mem2 : memory),
+      low_reg_mem_equiv priv_map (reg1, mem1) (reg2, mem2) ->
+      low_reg_mem_equiv priv_map (reg1, update x v mem1) (reg2, mem2).
+Proof.
+  intros priv_map x v Hx reg1 mem1 reg2 mem2 Hs.
+  red. red in Hs. intros. unfold update.
+  assert (x <> x0).
+  { intro. subst. rewrite Hx in H. discriminate. }
+  apply eqb_neq in H0. rewrite H0. auto.
+Qed.
+
+Lemma low_reg_mem_equiv_update_priv_r:
+  forall (priv_map : privacy_map) (x : addr) (v : value),
+    priv_map x = Private ->
+    forall (reg1 : registers) (mem1 : memory) (reg2 : registers) (mem2 : memory),
+      low_reg_mem_equiv priv_map (reg1, mem1) (reg2, mem2) ->
+      low_reg_mem_equiv priv_map (reg1, mem1) (reg2, update x v mem2).
+Proof.
+  intros priv_map x v Hx reg1 mem1 reg2 mem2 Hs.
+  red. red in Hs. intros. unfold update.
+  assert (x <> x0).
+  { intro. subst. rewrite Hx in H. discriminate. }
+  apply eqb_neq in H0. rewrite H0. auto.
+Qed.
